boogie: Basic handling of type constructors and constants

test/control-flow/procedure.bpl
@@ -1,13 +1,11 @@
 // RUN: %boogie "%s" > "%t"
 // RUN: %diff "%s".expect "%t"
 
-
 procedure p0(x: int, y: int) returns (z: int) requires true ; ensures z == 5;
 {
     z := 5;
     return;
 }
-
 
 procedure main() returns () {
     var z: int;
@@ -17,3 +15,65 @@ procedure main() returns () {
 
 }
 
+// From test2/Call: Parameters for the procedures have been renamed
+// since the haskell backed doesn't support substitution
+
+procedure Bar() returns (barresult: ref);
+
+procedure Foo();
+
+implementation Foo()
+{
+  var x: ref;
+
+  entry:
+    call x := Bar();
+    assume x == null;
+    call x := Bar();
+    assert x == null; // error
+    return;
+
+}
+
+procedure DifferentFormalNames(x: int, y: int) returns (z: int);
+  requires x < y;
+  ensures z == x;
+
+implementation DifferentFormalNames(x: int, y: int) returns (z: int)
+{
+  start:
+    assert x < y;
+    z := x;
+    return;
+}
+
+implementation DifferentFormalNames(x: int, y: int) returns (z: int)
+{
+  start:
+    goto A, B;
+  A:
+    assert x < y;
+    assume false;
+    return;
+  B:
+    z := x;
+    return;
+}
+
+implementation DifferentFormalNames(x: int, y: int) returns (z: int)
+{
+  start:
+    assert y < x;  // error
+    z := x;
+    return;
+}
+
+implementation DifferentFormalNames(x: int, y: int) returns (z: int)
+{
+  start:
+    z := y;
+    return;  // error: postcondition violation
+}
+
+type ref;
+const null : ref;
